src/Bedrock/Field/Interface/Compilation2.v
@@ -268,7 +268,7 @@ Section Compile.
   Local Hint Extern 1 (spec_of _) => (simple refine (@spec_of_from_word _ _ _ _ _ _ _ _)) : typeclass_instances.
 
   Lemma compile_from_word {tr m l functions} x:
-    let v := F.of_Z _ x in
+    let v := Zmod.of_Z _ x in
     forall P (pred: P v -> predicate) (k: nlet_eq_k P v) k_impl
            R (wx : word) out out_ptr out_var out_bounds,
 
@@ -354,7 +354,7 @@ Section Compile.
   Qed.
 
   Lemma compile_to_bytes {tr m l functions} x :
-    let v : list _ := Z_to_bytes (F.to_Z x) encoded_felem_size_in_bytes in
+    let v : list _ := Z_to_bytes (Zmod.unsigned x) encoded_felem_size_in_bytes in
     forall P (pred: P v -> predicate) (k: nlet_eq_k P v) k_impl
            Rx R x_ptr x_var out out_ptr out_var,
 
@@ -407,18 +407,18 @@ End Compile.
 
 
 (*must be higher priority than compile_mul*)
-#[export] Hint Extern 6 (WeakestPrecondition.cmd _ _ _ _ _ (_ (nlet_eq _ (a24 * _)%F _))) =>
+#[export] Hint Extern 6 (WeakestPrecondition.cmd _ _ _ _ _ (_ (nlet_eq _ (a24 * _)%Zmod _))) =>
 simple eapply compile_scmula24; shelve : compiler.
 
-#[export] Hint Extern 8 (WeakestPrecondition.cmd _ _ _ _ _ (_ (nlet_eq _ (_ * _)%F _))) =>
+#[export] Hint Extern 8 (WeakestPrecondition.cmd _ _ _ _ _ (_ (nlet_eq _ (_ * _)%Zmod _))) =>
 simple eapply compile_mul; shelve : compiler.
-#[export] Hint Extern 8 (WeakestPrecondition.cmd _ _ _ _ _ (_ (nlet_eq _ (_ + _)%F _))) =>
+#[export] Hint Extern 8 (WeakestPrecondition.cmd _ _ _ _ _ (_ (nlet_eq _ (_ + _)%Zmod _))) =>
 simple eapply compile_add; shelve : compiler.
-#[export] Hint Extern 8 (WeakestPrecondition.cmd _ _ _ _ _ (_ (nlet_eq _ (_ - _)%F _))) =>
+#[export] Hint Extern 8 (WeakestPrecondition.cmd _ _ _ _ _ (_ (nlet_eq _ (_ - _)%Zmod _))) =>
 simple eapply compile_sub; shelve : compiler.
-#[export] Hint Extern 8 (WeakestPrecondition.cmd _ _ _ _ _ (_ (nlet_eq _ (_ ^ 2)%F _))) =>
+#[export] Hint Extern 8 (WeakestPrecondition.cmd _ _ _ _ _ (_ (nlet_eq _ (_ ^ 2)%Zmod _))) =>
 simple eapply compile_square; shelve : compiler.
-#[export] Hint Extern 8 (WeakestPrecondition.cmd _ _ _ _ _ (_ (nlet_eq _ (F.of_Z _ _) _))) =>
+#[export] Hint Extern 8 (WeakestPrecondition.cmd _ _ _ _ _ (_ (nlet_eq _ (Zmod.of_Z _ _) _))) =>
 simple eapply compile_from_word; shelve : compiler.
 #[export] Hint Extern 10 (WeakestPrecondition.cmd _ _ _ _ _ (_ (nlet_eq _ ?v _))) =>
 is_var v; simple eapply compile_felem_copy; shelve : compiler.
