src/Bedrock/Group/ScalarMult/LadderStep.v
@@ -5,10 +5,10 @@ Require Import Crypto.Bedrock.Field.Interface.Compilation2.
 Local Open Scope Z_scope.
 
 Section Gallina.
-  Local Open Scope F_scope.
+  Local Open Scope Zmod_scope.
 
-  Definition ladderstep_gallina (m : Z) (a24 : F m)
-             (X1 X2 Z2 X3 Z3: F m) : \<< F m, F m, F m, F m \>> :=
+  Definition ladderstep_gallina (m : Z) (a24 : Zmod m)
+             (X1 X2 Z2 X3 Z3: Zmod m) : \<< Zmod m, Zmod m, Zmod m, Zmod m \>> :=
     let/n A := stack (X2+Z2) in
     let/n X2 := (X2-Z2) in
     let/n Z2 := (X3+Z3) in
@@ -46,7 +46,7 @@ Section __.
   Instance spec_of_ladderstep : spec_of "ladderstep" :=
     fnspec! "ladderstep"
           (pX1 pX2 pZ2 pX3 pZ3 : word)
-          / (X1 X2 Z2 X3 Z3 : F M) R,
+          / (X1 X2 Z2 X3 Z3 : Zmod M) R,
     { requires tr mem :=
         (FElem (Some tight_bounds) pX1 X1
          * FElem (Some tight_bounds) pX2 X2
@@ -56,7 +56,7 @@ Section __.
       ensures tr' mem' :=
         tr = tr'
         /\ exists X4 Z4 X5 Z5 (* output values *)
-                  : F M,
+                  : Zmod M,
                   (ladderstep_gallina M a24 X1 X2 Z2 X3 Z3
            = \<X4, Z4, X5, Z5\>)
           /\ (FElem (Some tight_bounds) pX1 X1
@@ -66,7 +66,7 @@ Section __.
               * FElem (Some tight_bounds) pZ3 Z5 * R)%sep mem'}.
 
   Lemma compile_ladderstep {tr m l functions}
-        (x1 x2 z2 x3 z3 : F M) :
+        (x1 x2 z2 x3 z3 : Zmod M) :
     let v := ladderstep_gallina M a24 x1 x2 z2 x3 z3 in
     forall P (pred: P v -> predicate) (k: nlet_eq_k P v) k_impl
            Rout
